examples/ghc/module-edits/OccName/midamble.v
@@ -3,3 +3,42 @@ Require Import Module.
 
 Instance Uniquable_OccName : Unique.Uniquable OccName := {}.
 Admitted.
+
+Definition compare_Namespace : NameSpace -> NameSpace -> comparison :=
+  fun x y => match x , y with
+          | VarName   , VarName   => Eq
+          | VarName   , _         => Lt
+          | _         , VarName   => Gt
+          | DataName  , DataName  => Eq
+          | _         , DataName  => Lt
+          | DataName  , _         => Gt
+          | TvName    , TvName    => Eq
+          | _         , TvName    => Lt
+          | TvName    , _         => Gt
+          | TcClsName , TcClsName => Eq
+          end.
+
+Local Definition NameSpace_op_zg__ : NameSpace -> NameSpace -> bool :=
+  fun x y => match compare_Namespace x y with
+            | Gt => true
+            | _  => false
+          end.
+
+Local Definition NameSpace_op_zgze__ : NameSpace -> NameSpace -> bool :=
+  fun x y => match compare_Namespace x y with
+            | Gt => true
+            | Eq => true
+            | _  => false
+          end.
+
+Local Definition NameSpace_op_zl__ : NameSpace -> NameSpace -> bool :=
+  fun x y => match compare_Namespace x y with
+            | Lt => true
+            | _  => false
+          end.
+Local Definition NameSpace_op_zlze__ : NameSpace -> NameSpace -> bool :=
+  fun x y => match compare_Namespace x y with
+            | Lt => true
+            | Eq => true
+            | _  => false
+          end.
