examples/ghc/lib/UniqFM.v
@@ -31,7 +31,13 @@ Arguments UFM {_} _.
 (* Midamble *)
 
 Require Data.IntSet.Base.
+
 Axiom ufmToSet_Directly : forall {elt}, UniqFM elt -> Data.IntSet.Base.IntSet.
+
+Require Panic.
+
+Instance Default_UniqFM {a} : Panic.Default (UniqFM a) :=
+  Panic.Build_Default _ (UFM Data.IntMap.Base.empty).
 
 (* Converted value declarations: *)
 
