examples/ghc/module-edits/UniqFM/midamble.v
@@ -1,2 +1,8 @@
 Require Data.IntSet.Base.
+
 Axiom ufmToSet_Directly : forall {elt}, UniqFM elt -> Data.IntSet.Base.IntSet.
+
+Require Panic.
+
+Instance Default_UniqFM {a} : Panic.Default (UniqFM a) :=
+  Panic.Build_Default _ (UFM Data.IntMap.Base.empty).
